caca

plop.v
@@ -1,4 +1,67 @@
 Require Import List Arith.
+Require Import FSets FSetAVL FSetFacts FSetEqProperties FSetProperties.
+Module Nat <: OrderedType.
+  Definition t := nat.
+  Definition eq (a b : t) := a=b.
+  Definition lt (a b : t) := a<b.
+
+  Lemma eq_refl : forall x : t, eq x x.
+  Proof.
+    intro;unfold eq;auto.
+  Qed.
+
+  Lemma eq_sym : forall x y : t, eq x y -> eq y x.
+  Proof.
+    intro;unfold eq;auto.
+  Qed.
+
+  Lemma eq_trans : forall x y z : t, eq x y -> eq y z -> eq x z.
+  Proof.
+    intros x y z h h';unfold eq in *; rewrite h in *;auto.
+  Qed.
+
+  Definition lt_trans : forall x y z : t, lt x y -> lt y z -> lt x z :=
+    lt_trans.
+
+  Definition lt_not_eq : forall x y : t, lt x y -> ~ eq x y :=
+    NPeano.Nat.lt_neq.
+  
+  Definition compare : forall x y : t, Compare lt eq x y.
+  Proof.
+    SearchAbout ({ _ } +  { _ } + { _ } ).
+    intros x y; case (lt_eq_lt_dec x y) as [[h|h]|h];
+    [apply LT
+    |apply EQ
+    |apply GT];auto.
+  Qed.
+  Definition eq_dec := eq_nat_dec.
+End Nat.
+
+Module NSet := FSetAVL.Make(Nat).
+Module NF := FSetFacts.Facts NSet.
+Module NP := FSetProperties.Properties NSet.
+
+Lemma Equal_add : forall x s s', NSet.eq s s' ->
+                                 NSet.eq (NSet.add x s) (NSet.add x s').
+Proof.
+  intros x s s' he.
+  apply NP.Add_Equal;simpl; intro y;
+  case (eq_nat_dec x y) as [->|h];split;intro h';
+  [left
+  |apply NSet.add_1
+  |right;apply he;apply NSet.add_3 in h'
+  |case h' as [->|h'];
+    [absurd (y = y)
+    |apply NSet.add_2;apply he]
+  ]; auto.
+Qed.
+
+Inductive Sousmot : list nat -> list nat -> Prop :=
+| sempty v : Sousmot nil v
+| scons1 x u v : Sousmot u v -> Sousmot u (x::v)
+| scons2 x u v : Sousmot u v -> Sousmot (x::u) (x::v).
+
+
 
 Variable L : nat.
 
@@ -53,9 +116,8 @@ Proof.
   [ assumption
   | apply h1].
 Qed.
-
-Definition memory := (list nat) %type.
-Definition disk := list nat.
+Definition memory := NSet.t.
+Definition disk := NSet.t.
 Definition buffer := nat.
 Definition state := (buffer * buffer * memory * disk) %type.
 Definition get_top (e : state) :=
@@ -67,23 +129,17 @@ Definition get_memory (e : state) :=
 Definition get_disk (e : state) :=
   match e with (t,b,m,d) => d end.
 
-Definition same_elts {A} l m :=
-  forall a : A, In a l <-> In a m.
-
-Definition same_elts_upto i l m :=
-  forall a, a < i -> (In a l <-> In a m).
-
 Definition equiv e f :=
   get_top e = get_top f
   /\ get_bottom e = get_bottom f
-  /\ same_elts (get_memory e) (get_memory f)
-  /\ same_elts (get_disk e) (get_disk f).
+  /\ NSet.eq (get_memory e) (get_memory f)
+  /\ NSet.eq (get_disk e) (get_disk f).
 
-Definition equiv_upto e f :=
+(*Definition equiv_upto e f :=
   get_top e = get_top f
   /\ get_bottom e = get_bottom f
   /\ same_elts_upto (get_bottom e) (get_memory e) (get_memory f)
-  /\ same_elts_upto (get_bottom e) (get_disk e) (get_disk f).
+  /\ same_elts_upto (get_bottom e) (get_disk e) (get_disk f).*)
 
 Notation "e ≡ f" := (equiv e f) (at level 20). (*need to understand 20*)
 
@@ -98,11 +154,7 @@ Lemma equiv_sym e f :
 Proof.
 intro H. destruct H as (h0 & h1 & h2 & h3).
 unfold equiv; rewrite h1 in *.
- repeat split; intros; auto;
- [ apply h2
- | apply h2
- | apply h3
- | apply h3]; auto.
+split ; [|split;[|split]];auto;apply NSet.eq_sym; auto.
 Qed.
 
 Lemma equiv_trans f e g :
@@ -110,16 +162,15 @@ Lemma equiv_trans f e g :
 Proof.
 intros (h0 & h1 & h2 & h3) (hh0 & hh1 & hh2 & hh3).
 unfold equiv; rewrite h0 in *.
-rewrite h1 in *; rewrite hh1 in *.
-repeat split; auto; intros. 
-apply hh2; auto; apply h2; auto.
-apply h2; auto; apply hh2; auto.
-apply hh3; auto; apply h3; auto.
-apply h3; auto; apply hh3; auto.
+rewrite h1 in *; rewrite h2 in *; rewrite h3 in *; rewrite hh1 in *.
+split ; [|split;[|split]];auto;apply NSet.eq_sym; auto.
 Qed.
 
 
-Definition size_memory e := length (get_memory e).
+Definition size_memory e := NSet.cardinal (get_memory e).
+
+Definition bound_memory e :=
+  size_memory e <= cmem.
 
 Definition rmv := remove (eq_nat_dec).
 
@@ -128,12 +179,12 @@ Definition eval_op e o : state :=
   match type o with
     | F => (i+1,get_bottom e,get_memory e,get_disk e)
     | Fb => (i,i,get_memory e, get_disk e)
-    | Wm => (i,get_bottom e,i::(get_memory e),get_disk e)
-    | Wd => (i,get_bottom e,get_memory e,i::(get_disk e))
+    | Wm => (i,get_bottom e,NSet.add i (get_memory e),get_disk e)
+    | Wd => (i,get_bottom e,get_memory e,NSet.add i (get_disk e))
     | Rm => (i,get_bottom e,get_memory e,get_disk e)
     | Rd => (i,get_bottom e,get_memory e,get_disk e)
-    | Dm => (get_top e,get_bottom e,rmv i (get_memory e),get_disk e)
-    | Dd => (get_top e,get_bottom e,get_memory e,rmv i (get_disk e))
+    | Dm => (get_top e,get_bottom e,NSet.remove i (get_memory e),get_disk e)
+    | Dd => (get_top e,get_bottom e,get_memory e,NSet.remove i (get_disk e))
   end.
   
 Definition eval_schedule e s :=
@@ -146,10 +197,10 @@ Definition valid_op e o : Prop :=
     | Fb => get_top e = i /\ get_bottom e = i+1
     | Wm => get_top e = i /\ size_memory e < cmem
     | Wd => get_top e = i
-    | Rm => In i (get_memory e)
-    | Rd => In i (get_disk e)
-    | Dm => In i (get_memory e)
-    | Dd => In i (get_disk e)
+    | Rm => NSet.In i (get_memory e)
+    | Rd => NSet.In i (get_disk e)
+    | Dm => NSet.In i (get_memory e)
+    | Dd => NSet.In i (get_disk e)
   end.
 
 Inductive valid_schedule : state -> schedule -> Prop :=
@@ -167,32 +218,82 @@ destruct o as (o & i); destruct o; simpl in *.
 
 rewrite <- h0; auto.
 rewrite <- h0; rewrite <- h1; auto.
-rewrite <- h0; rewrite <- h1; auto.
+destruct h as (h4 & h5c);
+  rewrite <- h0; split;
+  [|replace (size_memory f) with (size_memory e)];auto.
+apply NP.Equal_cardinal;auto.
+rewrite <- h0;auto.
+apply h2;auto.
+apply h3;auto.
+apply h2;auto.
+apply h3;auto.
+Qed.
 
+Lemma equiv_eval_op e f :
+  e ≡ f -> (forall o, eval_op e o ≡ eval_op f o ).
+Proof.
+  intros (h0 & h1& h2 & h3) (o & i); unfold eval_op; destruct o;simpl.
+  repeat (split;auto).  
+  repeat (split;auto).
+  split;[|split;[|split]];auto;apply Equal_add; auto. 
+  split;[|split;[|split]];auto;apply Equal_add; auto. 
+  repeat (split;auto).
+  repeat (split;auto).
+  split;[|split;[|split]];auto;apply NP.Equal_remove;auto. 
+  split;[|split;[|split]];auto;apply NP.Equal_remove;auto. 
 Qed.
 
 Lemma equiv_valid e f :
   e ≡ f -> (forall s, valid_schedule e s -> valid_schedule f s ).
 Proof.
-cut (forall s e f, e ≡ f -> valid_schedule e s -> valid_schedule f s).
-intros; auto.
-apply (H _ e); auto.
-induction s; intros; auto.
-inversion H0. discriminate.
-
+  cut (forall s e f, e ≡ f -> valid_schedule e s -> valid_schedule f s);
+  [ intros h1 h2 s;apply (h1 _ e);assumption
+  | induction s; intros e' f' h1 h2; 
+    [ apply vempty;reflexivity
+    | inversion h2;
+      [ discriminate
+      | apply vcons;
+        [ apply (equiv_valid_op e')
+        | apply (IHs (eval_op e' a));
+          [ apply equiv_eval_op
+          |
+          ]
+        ]
+      ];assumption
+    ]
+  ].
 Qed.
 
 Lemma equiv_eval e f :
   e ≡ f -> (forall s, eval_schedule e s ≡ eval_schedule f s ).
 Proof.
-Admitted.
-
+  cut (forall s e f, e ≡ f -> eval_schedule e s ≡ eval_schedule f s);
+  [intros h1 h2 s;apply (h1 _ e)
+  |induction s; intros e' f' h1;  unfold eval_schedule in * ; simpl;
+   [|apply IHs;apply equiv_eval_op]]; assumption.
+Qed.
 
 Lemma valid_app s1 s2 : forall e,
   valid_schedule e (s1 ++ s2) <->
   valid_schedule e s1 /\ valid_schedule (eval_schedule e s1) s2.
 Proof.
-induction s1; intro e; split; intro Hvs; auto. 
+  induction s1; intro e; split; intro Hvs.
+  simpl in *;split;[apply vempty;reflexivity|]; assumption.
+  
+  rewrite app_nil_l; destruct Hvs; simpl in *; assumption.
+
+  rewrite <- app_comm_cons in *; inversion Hvs;
+  [ discriminate
+  | apply IHs1 in H3; destruct H3;split;
+    [ apply vcons
+    | unfold eval_schedule in *;simpl]]; assumption.
+
+  rewrite <- app_comm_cons in *;destruct Hvs as (hvs1 & hvs2);
+  inversion hvs1; auto;[discriminate|];apply vcons;
+  [|rewrite IHs1; split];assumption.
+
+
+(*induction s1; intro e; split; intro Hvs; auto. 
 SearchAbout (nil ++ _). rewrite app_nil_l. destruct Hvs. simpl in *. assumption.
 rewrite <- app_comm_cons in *. inversion Hvs. 
 discriminate.
@@ -209,6 +310,7 @@ destruct Hvs as (hvs1 & hvs2). inversion hvs1; auto. discriminate. apply vcons.
 assumption.
 rewrite IHs1. split; auto.
 
+ *)
 Qed.
 
 Notation "[ a , b ]" := ((a,b)::nil) (at level 50).
@@ -237,7 +339,256 @@ Fixpoint remove_double_write_mem s :=
     | oi::s => oi::(remove_double_write_mem s)
   end.
 
+Lemma invert_rwmi s :
+  forall s1 s2 i,
+    remove_write_mem_i s i = s1 ++ s2 ->
+    (*~ In (Dm,i) s1 ->*)
+    (exists s3 s4, s=s3++s4 /\
+                     remove_write_mem_i s3 i = s1 /\
+                     remove_write_mem_i s4 i = s2)
+    \/ exists s3, s=s3++s2 /\
+                     remove_write_mem_i s3 i = s1.
+Proof.
+  induction s; intros s1 s2 i h; simpl in * .
+  destruct s1;destruct s2;
+  [simpl in *;left;exists nil; exists nil; repeat split;simpl
+  |contradict h;apply app_cons_not_nil
+  |simpl in h;discriminate
+  |simpl in h;discriminate].
+  set (x:=a);assert (x=a) as hx; [auto|rewrite hx in *].
+  destruct a as (o,k); destruct o; simpl in h;
+  try
+    (destruct s1;simpl in h;
+     [destruct s2;[discriminate
+                  |inversion h;left;exists nil; exists (x::s);
+                   repeat split;simpl]
+     |inversion h;
+       apply IHs in H1 as [(s3 & s4 & hs & hs3 & hs4)|(s3 & hs & hs3)]];
+     [left;exists (x::s3); exists s4;repeat split;simpl;
+      [f_equal|f_equal|]
+     |right;exists (x::s3); split;simpl;
+      [f_equal|f_equal]];assumption).
+  case (eq_nat_dec i k) as [-> |].
+  rewrite <- beq_nat_refl in h;
+    apply IHs in h as [(s3 & s4 & hs & hs3 & hs4)|(s3 & hs & hs3)];
+    [left;exists (x::s3); exists s4;repeat split;simpl;
+     [f_equal|rewrite <- beq_nat_refl|]
+    |right;exists (x::s3); split;simpl;
+     [f_equal|rewrite <- beq_nat_refl]];assumption.
 
+  replace (beq_nat i k) with false in h;
+    [|symmetry;apply beq_nat_false_iff;assumption].
+  destruct s1;simpl in h.
+  destruct s2;[discriminate
+                    |inversion h;left;exists nil; exists (x::s);
+                     repeat split;simpl];
+  replace (beq_nat i k) with false;
+    [|symmetry;apply beq_nat_false_iff;assumption];reflexivity.
+  inversion h.
+  apply IHs in H1 as [(s3 & s4 & hs & hs3 & hs4)|(s3 & hs & hs3)];
+    [left|right].
+  exists (x::s3);exists s4;repeat split;simpl;
+  [f_equal
+  |replace (beq_nat i k) with false;
+    [f_equal
+    |symmetry;apply beq_nat_false_iff]|];
+  assumption.
+  exists (x::s3); split;simpl;
+  [f_equal
+  |replace (beq_nat i k) with false;
+    [f_equal
+    |symmetry;apply beq_nat_false_iff]];
+  assumption.
+  case (eq_nat_dec i k) as [-> |].
+  rewrite <- beq_nat_refl in h.
+  destruct s1.
+  right; exists nil;split;[assumption|reflexivity].
+  right; exists (x::s1); split;[|rewrite hx; simpl;rewrite <- beq_nat_refl]; simpl in *;inversion h;f_equal.
+  replace (beq_nat i k) with false in h;
+    [|symmetry;apply beq_nat_false_iff;assumption].
+  destruct s1;simpl in h.
+  destruct s2;[discriminate
+                    |inversion h;left;exists nil; exists (x::s);
+                     repeat split;simpl];
+  replace (beq_nat i k) with false;
+    [|symmetry;apply beq_nat_false_iff;assumption];reflexivity.
+  inversion h.
+  apply IHs in H1 as [(s3 & s4 & hs & hs3 & hs4)|(s3 & hs & hs3)];
+    [left|right].
+  exists (x::s3);exists s4;repeat split;simpl;
+  [f_equal
+  |replace (beq_nat i k) with false;
+    [f_equal
+    |symmetry;apply beq_nat_false_iff]|];
+  assumption.
+  exists (x::s3); split;simpl;
+  [f_equal
+  |replace (beq_nat i k) with false;
+    [f_equal
+    |symmetry;apply beq_nat_false_iff]];
+  assumption.
+
+Qed.
+
+Lemma no_dwm_rdwmi s :
+  forall i j,
+    no_double_write_mem_i s i ->
+    no_double_write_mem_i (remove_write_mem_i s j) i.
+Proof.
+  assert (forall i s1 s2,remove_write_mem_i s1 i <> (Wm,i)::s2) as lem1.
+  induction s1 ;intros s2 h.
+  simpl in h; discriminate.
+  destruct a as (o,k); destruct o; simpl in h; try
+                                                   discriminate.
+  case (eq_nat_dec i k) as [ -> | ];
+  [rewrite <- beq_nat_refl in *
+  |replace (beq_nat i k) with false in *;
+    [|symmetry;apply beq_nat_false_iff;assumption]];
+  inversion h;[apply (IHs1 s2);assumption
+              |symmetry in H0;contradiction].  
+  case (eq_nat_dec i k) as [ -> | ];
+  [rewrite <- beq_nat_refl in *
+  |replace (beq_nat i k) with false in *;
+    [|symmetry;apply beq_nat_false_iff;assumption]];
+  discriminate.
+
+  assert (forall op k s1,
+           (remove_write_mem_i s1 k)= ->
+            In op s1) 
+    as lem2.
+  assert (forall op k s1,
+            In op (remove_write_mem_i s1 k) ->
+            In op s1) 
+    as lem2.
+  intros op i;induction s1;intro h;auto;
+  destruct a as (o,l); destruct o; simpl in *;
+  try (simpl;case (eq_nat_dec i l) as [ -> | ];
+    try (rewrite <- beq_nat_refl in *);
+    try (replace (beq_nat i l) with false in *);
+    try (symmetry;apply beq_nat_false_iff;assumption));
+  try case h as [<-|h];
+  try (left;reflexivity);
+  try (right;assumption);
+  try (right;apply IHs1;assumption).
+
+(*  assert (forall i k s1,
+             In (Dm,i) s1 ->
+             In (Dm,i)(remove_write_mem_i s1 k))
+    as lem3.*)
+  intros i j hs (s1 & s2 & s3 & h1 & h3).
+  apply invert_rwmi in h1 
+    as [(s4 & s5 & hs' & hs4 & hs5) | (s4 & hs' & hs4)].
+  apply invert_rwmi in hs5
+    as [(s6 & s7 & -> & hs6 & hs7) | (s6 & -> & hs6)].
+  apply invert_rwmi in hs7
+    as [(s8 & s9 & -> & hs8 & hs9) | (s8 & -> & hs8)].
+  apply invert_rwmi in hs9
+    as [(s10 & s11 & -> & hs10 & hs11) | (s10 & -> & hs10)].
+  
+  replace s6 with ([Wm,i]) in *.
+  replace s10 with ([Wm,i]) in *.
+
+  apply hs;exists s4; exists s8; exists s11.
+  split;[assumption|rewrite (lem2 _ j); rewrite hs8;assumption].
+  destruct s10.
+  simpl in hs10;discriminate.
+  
+  destruct s6;try (simpl in *;discriminate).
+  
+  
+  destruct s5;try (simpl in *;discriminate).
+  destruct p as (o,k); destruct o; simpl in hs5; try
+                                                   discriminate.
+  case (eq_nat_dec j k) as [-> | ]; 
+  [rewrite <- beq_nat_refl in *
+  |replace (beq_nat j k) with false in *;
+    [inversion hs5|symmetry;apply beq_nat_false_iff;assumption]].
+  replace ((Wm, i) :: s2 ++ (Wm, i) :: s3) with
+  (((Wm, i) :: s2) ++ (Wm, i) :: s3) in hs5;[|simpl;reflexivity]. 
+  apply invert_rwmi in hs5 
+    as [(s6 & s7 & -> & hs6 & hs7) | (s6 & -> & hs6)];
+  destruct s6;try (simpl in *;discriminate).
+  destruct p as (o,l); destruct o; simpl in hs6; try
+                                                   discriminate.
+  case (eq_nat_dec k l) as [ -> | h];
+  [rewrite <- beq_nat_refl in *
+  |replace (beq_nat k l) with false in *;
+    [inversion hs6|symmetry;apply beq_nat_false_iff;assumption]].
+
+  apply hs; exists s4;exists nil; exists (s6 ++ s7).
+split;simpl in *;[|].
+
+(*  induction s;
+  intros i j h  (s1 & s2 & s3 & h1 & h3).
+  apply (app_cons_not_nil s1 (s2 ++ (Wm, i) :: s3) (Wm,i));
+    simpl in h1;assumption.
+ apply invert_rwmi in h1 as [(s4 & s5 & hs & hs1 & hs2)
+                            | (s4 & hs & hs1)].*)
+  
+  intros i j h(*  (s1 & s2 & s3 & h1 & h3).
+  apply h*) .
+  induction s; intros (s1 & s2 & s3 & h1 & h3).
+  apply (app_cons_not_nil s1 (s2 ++ (Wm, i) :: s3) (Wm,i));
+    unfold no_double_write_mem_i in *; simpl in h1; auto.
+  assert (no_double_write_mem_i s i) as hs;
+    [intros (ss1 & ss2 & ss3 & hh1 & hh3);apply h;
+     exists (a::ss1);exists ss2;exists ss3;split;
+     [simpl;f_equal|];assumption| ].
+  
+  destruct a as (o,k); destruct o; simpl in h1;
+  try (apply IHs in hs;destruct s1 as [|(o & l)];
+       [discriminate|];
+       simpl in h1;inversion h1;apply hs;
+       exists s1;exists s2;exists s3;split;assumption).
+  case (eq_nat_dec j k) as [-> |].
+  rewrite <- beq_nat_refl in h1.
+  apply IHs in hs; apply hs; exists s1;exists s2;exists s3;split;
+  assumption.
+  replace (beq_nat j k) with false in h1;
+    [|symmetry;apply beq_nat_false_iff;assumption].
+  destruct s1 as [|(o & l)].
+  simpl in h1.
+  inversion h1.
+  apply invert_rwmi in H1 as [(s4 & s5 & hss & hs1 & hs2)
+                            | (s4 & hss & hs1)].
+  apply hs; exists nil;exists (remove_write_mem_i s2 j);exists (remove_write_mem_i s3 j).
+  split; [simpl|].
+  apply hs; exists nil;exists s2;exists s3.
+
+  [discriminate|];
+       simpl in h1;inversion h1;apply hs;
+       exists s1;exists s2;exists s3;split;assumption.
+Qed.
+  
+Lemma no_dwm_rdwm s :
+  forall i,
+    no_double_write_mem_i (remove_double_write_mem s) i.
+Proof.
+  induction s; unfold no_double_write_mem_i in *.
+  intros i (s1 & s2 & s3 & h1 & h3);simpl in h1.
+  apply (app_cons_not_nil s1 (s2 ++ (Wm, i) :: s3) (Wm,i)); auto.
+  intros i (s1 & s2 & s3 & h1 & h3).
+  destruct a as (o,j); destruct o; simpl in h1;
+  try 
+    (destruct s1 as [|(o & k)];
+     [discriminate|destruct o;simpl in h1;try discriminate;inversion h1];
+     apply (IHs i);exists s1; exists s2; exists s3;split;auto).
+  case (eq_nat_dec i j) as [<-| h].
+  Focus 2.
+  destruct s1 as [|(o & k)];  simpl in h1; inversion h1.
+  apply h; symmetry;assumption.
+  apply (IHs i);exists s1; exists s2; exists s3;split;auto.
+
+  [ 
+       |destruct o;simpl in h1;try discriminate;inversion h1];
+       apply (IHs i);exists s1; exists s2; exists s3;split;auto.
+
+  [|destruct s1 as [|(o & k)];  
+       [simpl in h1; inversion h1; apply h; symmetry;assumption
+       |destruct o;simpl in h1;try discriminate;inversion h1];
+       apply (IHs i);exists s1; exists s2; exists s3;split;auto].
+
+Qed.
 
 
 Lemma correct_rdwm s e :
@@ -250,8 +601,4 @@ Admitted.
 Lemma optimal_rdwm s e :
   optimal_schedule e s ->
   optimal_schedule e (remove_double_write_mem s).
-Admitted.
-Lemma no_dwm_rdwm s :
-  forall i,
-    no_double_write_mem_i (remove_double_write_mem s) i. 
 Admitted.
